\input{../header.tex}

\begin{document}
  \textbf{Bruchrechnen -  LÃ¶sung}\\\\
  Addition:\\\\
  $1+\frac{3}{2}=\frac{2}{2}+\frac{3}{2}=\frac{3+2}{2}=\frac{5}{2}$\\\\
  $\frac{4}{5}+\frac{1}{2}=\frac{8}{10}+\frac{5}{10}=\frac{8+5}{10}=\frac{13}{10}$\\\\
  $\frac{6}{3}+\frac{8}{2}=2+4=6$\\\\

  \noindent Subtraktion:\\\\
  $\frac{8}{9}-2=\frac{8}{9}-\frac{18}{9}=\frac{8-18}{9}=-\frac{10}{9}$\\\\
  $\frac{10}{7}-\frac{3}{7}=\frac{10-3}{7}=\frac{7}{7}=1$\\\\
  $\frac{-5}{24}-\frac{1}{6}=-\frac{5}{24}-\frac{4}{24}=\frac{-5-4}{24}=-\frac{9}{24}=-\frac{3}{8}$\\\\

  \noindent Multiplikation:\\\\
  $\frac{3}{4}\cdot\frac{2}{9}=\frac{3\cdot2}{2\cdot2\cdot3\cdot3}=\frac{1}{2\cdot3}=\frac{1}{6}$\\\\
  $28\cdot\frac{5}{7}=\frac{4\cdot7\cdot5}{7}=4\cdot5=20$\\\\
  $\frac{2}{13}\cdot\frac{26}{8}=\frac{2\cdot2\cdot13}{13\cdot2\cdot2\cdot2}=\frac{1}{2}$\\\\

  \noindent Division:\\\\
  $\frac{1}{2}:\frac{3}{4}=\frac{1}{2}\cdot\frac{4}{3}=\frac{1\cdot4}{2\cdot3}=\frac{2}{3}$\\\\
  $\frac{6}{5}:3=\frac{6}{5}\cdot\frac{1}{3}=\frac{2\cdot3}{5\cdot3}=\frac{2}{5}$\\\\
  $9:\frac{6}{2}=9\cdot\frac{2}{6}=9\cdot\frac{1}{3}=9:3=3$\\\\
\end{document}
